Tut 1
==============

# Q1

## d

* **(i)** $\forall a \in \mathbb{R} -(-a) = a$
* $\iff$ **(ii)** $-(-a) -a = 0$
* Proof of **(ii)**
  + $-(-a) -a = -(-a) + (-a)$ **Definition**
  + $=0$ **(A4)** 
 
## e

* **(i)** $(a+b) = -a -b$
* $\iff$ **(ii)** $$ -(a+b) +a + b = 0$
* Proof of **(ii)**
  + **(ii.i)** $-(a+b) + a + b = -(a+b) + (a + b)$ **(A1)** 
  + **(ii.ii)** $=0$ **(A4)**

## f

* **(i)** $0+0 = 0$ **(A3)**
* **(ii)** $a + b = 0 \iff b = -a$ **(A4) $\wedge$ b**
* **(iii)** $-0 = 0$ **(i),(ii)**

# Q2

## a

* **(i)** $a1 = a \quad a1' = a$ **(M3)**
* **(ii)** $a1 = a1'$ 
* **(iii)** $\, 1a = 1'a$ **(M2)**
* **(iv)** $\,1 a a^{-1} = 1' a a^{-1}$
* **(v)** $\,1 (a a^{-1}) = 1' (a a^{-1})$ **(M1)**
* **(vi)** $\quad 1 \cdot 1 = 1' \cdot 1$ **(M3)**
* **(vii)** $\quad 1 = 1'$ **So this is unique**

## b

* **(i)** $a a^{-1} = 1 \quad a (a^{-1})'$ **(M4)**
* **(ii)** $aa^{-1} = a(a^{-1})'$
* **(iii)** $a^{-1}a = (a^{-1})'a$ **(M2)**
* **(iv)** $a^{-1}a a^{-1} = (a^{-1})' a a^-1$
* **(v)** $a^{-1}(a a^{-1}) = (a^{-1})' (a a^-1)$ **(M1)**
* **(vi)** $a^{-1} 1 = (a^{-1})' 1$ **(M4)**
* **(vii)** $^a{-1} = (a^{-1})'$ **(M3)** **Unique** 

## c

* **(i)** $ax = b \quad ax' = b$ **2 solutions to the equaiton**
* **(ii)** $ax = ax'$
* **(iii)** $xa = x'a$ **(M2)**
* **(iv)** $xaa^{-1} =x' a a^{-1}$
* **(v)** $x(aa^{-1} )=  x'(a a^{-1})$  **(M1)**
* **(vi)** $x1= x'1$ **(M4)**
* **(vii)** $x = x'$ **(M3)** **Unique**

## d

* **(i)** $1 = 1$
* **(ii)** $(a^{-1})(a^{-1})^{-1} = a a^{-1}$ **(M4)** **$\neq 0$**
* **(iii)** $a a^{-1} (a^{-1})^{-1} = a a a^{-1}$
* **(iv)** $(a a^{-1}) (a^{-1})^{-1} = a (a a^{-1}$ **(M2)**
* **(v)** $\,1 (a^{-1})^{-1} = a 1$ **(M4)**
* **(vi)** $(a^{1})^{-1} 1 = a 1$ **(M2)**
* **(vii)** $(a^{-1})^{-1} = a$ **(M3)**

## e

* **(i)** $1 = 1$
* **(ii)** $(ab)(ab)^{-1} = a a^{-1} = a a{-1} b b^{-1}$ **(M4)**
* **(iii)** $(ab)^{-1}(ab) = a^{-1} b^{-1} ab = a^{-1} b^{-1} (ab)$ **(M1,M2) **
* **(iv)** $(ab)^{-1}(ab)(ab)^{-1} = a^{-1}b^{-1} (ab) (ab)^{-1}$
* **(v)** $(ab)^{-1} 1 = a^{-1} b^{-1} 1$ **(M4)**
* **(vi)** $(ab)^{-1} = a^{-1} b^{-1}$ **(M3)** 

## f

* **(i)** $(-a)^{-1} = -a^{-1}$
* $\iff$ **(ii)** $(-a)(-a)^{-1} = (-a)-a^{-1}$
* $\iff$ **(iii)** $\, 1 = (-1) (-1) a a^{-1}$ **(Theorem 1.2 e, M2)**
* **(iv)** $\,1 = 1$ **(Theorem 1.2 f, M4)**

## g

* **(i)** $1 \cdot 1 = 1$ **(M3)**
* **(ii)** $\,1^{-1} =1$ **(M4, b)**

## Q3

#. A rational number is any number that can be formed by deviding one integer by a none zero integer
      + All axioms exept completness


#. $x = \frac{x_1}{x_2} \quad x_1,x_2 \in \mathbb{Z} \quad y = \frac{y_1}{y_2} \quad y \in \mathbb{Z} \neq0$
  * $x + y = \frac{x_1y_2 + x_2y_1}{x_2y_2}$ Both top and bottom are intgegers as integers are closed under addition and multiplication so the sum is a rational number
  * $x + y = \frac{x_1y_2}{x_2y_2}$ **Same reasoning**

# 4

## 1

* $(a + b) -c$
* $= a + b -c$ **(A1)**
* $= a + b + (-c)$ **Def**
* $= a + (b+(-c))$ **(A1)**
* $= a + (b-c)$ **Def**

## 2

* $a - (b-c)$
* $= a + (-1)(b) +(-1)(-c)$ **Theorem 1.2 e, D**
* $= a + (-1)(-c) + (-1)(b)$ **(A1)**
* $= a + c - b$ **(Theorem 1.2 e and f)**
* $= (c + a) -b$ **(A1 A2)**

## 3

* $a((2b + 1) + 3)$
* $a(2b + 1) + a3$ **D**
* $a2b + a + 3a$ **D, M2**
* $2ab + 1a + 3a$ **M2 M3**
* $2ab + (1+3)a$ **D** = 2ab +4a$ 

## 4

* $(-a)b$
* $=b(-a)$ **(M2)** 
 


