\PassOptionsToPackage{unicode=true}{hyperref} % options for packages loaded elsewhere
\PassOptionsToPackage{hyphens}{url}
%
\documentclass[]{article}
\usepackage{lmodern}
\usepackage{amssymb,amsmath}
\usepackage{ifxetex,ifluatex}
\usepackage{fixltx2e} % provides \textsubscript
\ifnum 0\ifxetex 1\fi\ifluatex 1\fi=0 % if pdftex
  \usepackage[T1]{fontenc}
  \usepackage[utf8]{inputenc}
  \usepackage{textcomp} % provides euro and other symbols
\else % if luatex or xelatex
  \usepackage{unicode-math}
  \defaultfontfeatures{Ligatures=TeX,Scale=MatchLowercase}
\fi
% use upquote if available, for straight quotes in verbatim environments
\IfFileExists{upquote.sty}{\usepackage{upquote}}{}
% use microtype if available
\IfFileExists{microtype.sty}{%
\usepackage[]{microtype}
\UseMicrotypeSet[protrusion]{basicmath} % disable protrusion for tt fonts
}{}
\IfFileExists{parskip.sty}{%
\usepackage{parskip}
}{% else
\setlength{\parindent}{0pt}
\setlength{\parskip}{6pt plus 2pt minus 1pt}
}
\usepackage{hyperref}
\hypersetup{
            pdfborder={0 0 0},
            breaklinks=true}
\urlstyle{same}  % don't use monospace font for urls
\setlength{\emergencystretch}{3em}  % prevent overfull lines
\providecommand{\tightlist}{%
  \setlength{\itemsep}{0pt}\setlength{\parskip}{0pt}}
\setcounter{secnumdepth}{0}
% Redefines (sub)paragraphs to behave more like sections
\ifx\paragraph\undefined\else
\let\oldparagraph\paragraph
\renewcommand{\paragraph}[1]{\oldparagraph{#1}\mbox{}}
\fi
\ifx\subparagraph\undefined\else
\let\oldsubparagraph\subparagraph
\renewcommand{\subparagraph}[1]{\oldsubparagraph{#1}\mbox{}}
\fi

% set default figure placement to htbp
\makeatletter
\def\fps@figure{htbp}
\makeatother


\date{}

\begin{document}

\hypertarget{tut-1}{%
\section{Tut 1}\label{tut-1}}

\hypertarget{q1}{%
\section{Q1}\label{q1}}

\hypertarget{d}{%
\subsection{d}\label{d}}

\begin{itemize}
\tightlist
\item
  \textbf{(i)} \(\forall a \in \mathbb{R} -(-a) = a\)
\item
  \(\iff\) \textbf{(ii)} \(-(-a) -a = 0\)
\item
  Proof of \textbf{(ii)}

  \begin{itemize}
  \tightlist
  \item
    \(-(-a) -a = -(-a) + (-a)\) \textbf{Definition}
  \item
    \(=0\) \textbf{(A4)}
  \end{itemize}
\end{itemize}

\hypertarget{e}{%
\subsection{e}\label{e}}

\begin{itemize}
\tightlist
\item
  \textbf{(i)} \((a+b) = -a -b\)
\item
  \(\iff\) \textbf{(ii)} \$\$ -(a+b) +a + b = 0\$
\item
  Proof of \textbf{(ii)}

  \begin{itemize}
  \tightlist
  \item
    \textbf{(ii.i)} \(-(a+b) + a + b = -(a+b) + (a + b)\) \textbf{(A1)}
  \item
    \textbf{(ii.ii)} \(=0\) \textbf{(A4)}
  \end{itemize}
\end{itemize}

\hypertarget{f}{%
\subsection{f}\label{f}}

\begin{itemize}
\tightlist
\item
  \textbf{(i)} \(0+0 = 0\) \textbf{(A3)}
\item
  \textbf{(ii)} \(a + b = 0 \iff b = -a\) \textbf{(A4) \(\wedge\) b}
\item
  \textbf{(iii)} \(-0 = 0\) \textbf{(i),(ii)}
\end{itemize}

\hypertarget{q2}{%
\section{Q2}\label{q2}}

\hypertarget{a}{%
\subsection{a}\label{a}}

\begin{itemize}
\tightlist
\item
  \textbf{(i)} \(a1 = a \quad a1' = a\) \textbf{(M3)}
\item
  \textbf{(ii)} \(a1 = a1'\)
\item
  \textbf{(iii)} \(\, 1a = 1'a\) \textbf{(M2)}
\item
  \textbf{(iv)} \(\,1 a a^{-1} = 1' a a^{-1}\)
\item
  \textbf{(v)} \(\,1 (a a^{-1}) = 1' (a a^{-1})\) \textbf{(M1)}
\item
  \textbf{(vi)} \(\quad 1 \cdot 1 = 1' \cdot 1\) \textbf{(M3)}
\item
  \textbf{(vii)} \(\quad 1 = 1'\) \textbf{So this is unique}
\end{itemize}

\hypertarget{b}{%
\subsection{b}\label{b}}

\begin{itemize}
\tightlist
\item
  \textbf{(i)} \(a a^{-1} = 1 \quad a (a^{-1})'\) \textbf{(M4)}
\item
  \textbf{(ii)} \(aa^{-1} = a(a^{-1})'\)
\item
  \textbf{(iii)} \(a^{-1}a = (a^{-1})'a\) \textbf{(M2)}
\item
  \textbf{(iv)} \(a^{-1}a a^{-1} = (a^{-1})' a a^-1\)
\item
  \textbf{(v)} \(a^{-1}(a a^{-1}) = (a^{-1})' (a a^-1)\) \textbf{(M1)}
\item
  \textbf{(vi)} \(a^{-1} 1 = (a^{-1})' 1\) \textbf{(M4)}
\item
  \textbf{(vii)} \(^a{-1} = (a^{-1})'\) \textbf{(M3)} \textbf{Unique}
\end{itemize}

\hypertarget{c}{%
\subsection{c}\label{c}}

\begin{itemize}
\tightlist
\item
  \textbf{(i)} \(ax = b \quad ax' = b\) \textbf{2 solutions to the
  equaiton}
\item
  \textbf{(ii)} \(ax = ax'\)
\item
  \textbf{(iii)} \(xa = x'a\) \textbf{(M2)}
\item
  \textbf{(iv)} \(xaa^{-1} =x' a a^{-1}\)
\item
  \textbf{(v)} \(x(aa^{-1} )= x'(a a^{-1})\) \textbf{(M1)}
\item
  \textbf{(vi)} \(x1= x'1\) \textbf{(M4)}
\item
  \textbf{(vii)} \(x = x'\) \textbf{(M3)} \textbf{Unique}
\end{itemize}

\hypertarget{d-1}{%
\subsection{d}\label{d-1}}

\begin{itemize}
\tightlist
\item
  \textbf{(i)} \(1 = 1\)
\item
  \textbf{(ii)} \((a^{-1})(a^{-1})^{-1} = a a^{-1}\) \textbf{(M4)}
  \textbf{\(\neq 0\)}
\item
  \textbf{(iii)} \(a a^{-1} (a^{-1})^{-1} = a a a^{-1}\)
\item
  \textbf{(iv)} \((a a^{-1}) (a^{-1})^{-1} = a (a a^{-1}\) \textbf{(M2)}
\item
  \textbf{(v)} \(\,1 (a^{-1})^{-1} = a 1\) \textbf{(M4)}
\item
  \textbf{(vi)} \((a^{1})^{-1} 1 = a 1\) \textbf{(M2)}
\item
  \textbf{(vii)} \((a^{-1})^{-1} = a\) \textbf{(M3)}
\end{itemize}

\hypertarget{e-1}{%
\subsection{e}\label{e-1}}

\begin{itemize}
\tightlist
\item
  \textbf{(i)} \(1 = 1\)
\item
  \textbf{(ii)} \((ab)(ab)^{-1} = a a^{-1} = a a{-1} b b^{-1}\)
  \textbf{(M4)}
\item
  \textbf{(iii)}
  \((ab)^{-1}(ab) = a^{-1} b^{-1} ab = a^{-1} b^{-1} (ab)\)
  \textbf{(M1,M2) }
\item
  \textbf{(iv)} \((ab)^{-1}(ab)(ab)^{-1} = a^{-1}b^{-1} (ab) (ab)^{-1}\)
\item
  \textbf{(v)} \((ab)^{-1} 1 = a^{-1} b^{-1} 1\) \textbf{(M4)}
\item
  \textbf{(vi)} \((ab)^{-1} = a^{-1} b^{-1}\) \textbf{(M3)}
\end{itemize}

\hypertarget{f-1}{%
\subsection{f}\label{f-1}}

\begin{itemize}
\tightlist
\item
  \textbf{(i)} \((-a)^{-1} = -a^{-1}\)
\item
  \(\iff\) \textbf{(ii)} \((-a)(-a)^{-1} = (-a)-a^{-1}\)
\item
  \(\iff\) \textbf{(iii)} \(\, 1 = (-1) (-1) a a^{-1}\) \textbf{(Theorem
  1.2 e, M2)}
\item
  \textbf{(iv)} \(\,1 = 1\) \textbf{(Theorem 1.2 f, M4)}
\end{itemize}

\hypertarget{g}{%
\subsection{g}\label{g}}

\begin{itemize}
\tightlist
\item
  \textbf{(i)} \(1 \cdot 1 = 1\) \textbf{(M3)}
\item
  \textbf{(ii)} \(\,1^{-1} =1\) \textbf{(M4, b)}
\end{itemize}

\hypertarget{q3}{%
\subsection{Q3}\label{q3}}

\begin{enumerate}
\tightlist
\item
  A rational number is any number that can be formed by deviding one
  integer by a none zero integer

  \begin{itemize}
  \tightlist
  \item
    All axioms exept completness
  \end{itemize}
\item
  \(x = \frac{x_1}{x_2} \quad x_1,x_2 \in \mathbb{Z} \quad y = \frac{y_1}{y_2} \quad y \in \mathbb{Z} \neq0\)
\end{enumerate}

\begin{itemize}
\tightlist
\item
  \(x + y = \frac{x_1y_2 + x_2y_1}{x_2y_2}\) Both top and bottom are
  intgegers as integers are closed under addition and multiplication so
  the sum is a rational number
\item
  \(x + y = \frac{x_1y_2}{x_2y_2}\) \textbf{Same reasoning}
\end{itemize}

\hypertarget{section}{%
\section{4}\label{section}}

\hypertarget{section-1}{%
\subsection{1}\label{section-1}}

\begin{itemize}
\tightlist
\item
  \((a + b) -c\)
\item
  \(= a + b -c\) \textbf{(A1)}
\item
  \(= a + b + (-c)\) \textbf{Def}
\item
  \(= a + (b+(-c))\) \textbf{(A1)}
\item
  \(= a + (b-c)\) \textbf{Def}
\end{itemize}

\hypertarget{section-2}{%
\subsection{2}\label{section-2}}

\begin{itemize}
\tightlist
\item
  \(a - (b-c)\)
\item
  \(= a + (-1)(b) +(-1)(-c)\) \textbf{Theorem 1.2 e, D}
\item
  \(= a + (-1)(-c) + (-1)(b)\) \textbf{(A1)}
\item
  \(= a + c - b\) \textbf{(Theorem 1.2 e and f)}
\item
  \(= (c + a) -b\) \textbf{(A1 A2)}
\end{itemize}

\hypertarget{section-3}{%
\subsection{3}\label{section-3}}

\begin{itemize}
\tightlist
\item
  \(a((2b + 1) + 3)\)
\item
  \(a(2b + 1) + a3\) \textbf{D}
\item
  \(a2b + a + 3a\) \textbf{D, M2}
\item
  \(2ab + 1a + 3a\) \textbf{M2 M3}
\item
  \(2ab + (1+3)a\) \textbf{D} = 2ab +4a\$
\end{itemize}

\hypertarget{section-4}{%
\subsection{4}\label{section-4}}

\begin{itemize}
\tightlist
\item
  \((-a)b\)
\item
  \(=b(-a)\) \textbf{(M2)}
\end{itemize}

\end{document}
